wip omnismall

ln/STLC_Ref_Definitions.v
@@ -4,7 +4,7 @@
 ***************************************************************************)
 
 Set Implicit Arguments.
-From TLC Require Import LibLN.
+From TLC Require Export LibLN.
 
 
 (* ********************************************************************** *)
@@ -17,9 +17,12 @@ Inductive typ : Set :=
   | typ_var   : var -> typ
   | typ_arrow : typ -> typ -> typ
   | typ_ref   : typ -> typ
+  | typ_int   : typ
   | typ_unit  : typ.
 
-(** Grammar of pre-terms. *)
+(** Grammar of pre-terms. For simplicity, integers are restricted to naturals. *)
+
+Definition int := nat.
 
 Definition loc := var.
 
@@ -29,10 +32,12 @@ Inductive trm : Set :=
   | trm_abs  : trm -> trm
   | trm_app  : trm -> trm -> trm
   | trm_unit : trm
+  | trm_int : int -> trm
   | trm_loc : loc -> trm
   | trm_ref : trm -> trm
   | trm_get : trm -> trm
-  | trm_set : trm -> trm -> trm.
+  | trm_set : trm -> trm -> trm
+  | trm_rand : trm -> trm.
 
 (** Opening up abstractions *)
 
@@ -42,11 +47,13 @@ Fixpoint open_rec (k : nat) (u : trm) (t : trm) {struct t} : trm :=
   | trm_fvar x    => trm_fvar x
   | trm_abs t1    => trm_abs (open_rec (S k) u t1)
   | trm_app t1 t2 => trm_app (open_rec k u t1) (open_rec k u t2)
-  | trm_unit          => trm_unit
+  | trm_unit      => trm_unit
+  | trm_int n     => trm_int n
   | trm_loc l     => trm_loc l
   | trm_ref t1    => trm_ref (open_rec k u t1)
   | trm_get t1    => trm_get (open_rec k u t1)
   | trm_set t1 t2 => trm_set (open_rec k u t1) (open_rec k u t2)
+  | trm_rand t1   => trm_rand (open_rec k u t1)
   end.
 
 Definition open t u := open_rec 0 u t.
@@ -67,9 +74,11 @@ Inductive term : trm -> Prop :=
       term t1 -> term t2 -> term (trm_app t1 t2)
   | term_trm_unit :
       term trm_unit
+  | term_int : forall n,
+      term (trm_int n)
   | term_loc : forall l,
       term (trm_loc l)
-  | term_new : forall t1,
+  | term_ref : forall t1,
       term t1 ->
       term (trm_ref t1)
   | term_get : forall t1,
@@ -78,7 +87,10 @@ Inductive term : trm -> Prop :=
   | term_set : forall t1 t2,
       term t1 ->
       term t2 ->
-      term (trm_set t1 t2).
+      term (trm_set t1 t2)
+  | term_rand : forall t1,
+      term t1 ->
+      term (trm_rand t1).
 
 (** Store maps (sto) locations to values, and
     Store typing (phi) maps locations to type. *)
@@ -101,50 +113,55 @@ Definition env := LibEnv.env typ.
 
 (** Typing relation *)
 
-Reserved Notation "E ! P |= t ~: T" (at level 69).
+Reserved Notation "E ! Y |= t ~: T" (at level 69).
 
 Inductive typing : env -> phi -> trm -> typ -> Prop :=
-  | typing_var : forall E P x T,
+  | typing_var : forall E Y x T,
       ok E ->
       binds x T E ->
-      E ! P |= (trm_fvar x) ~: T
-  | typing_abs : forall L E P U T t1,
-      (forall x, x \notin L -> (E & x ~ U) ! P  |= t1 ^ x ~: T) ->
-      E ! P |= (trm_abs t1) ~: (typ_arrow U T)
-  | typing_app : forall S T E P t1 t2,
-      E ! P |= t1 ~: (typ_arrow S T) -> E ! P  |= t2 ~: S ->
-      E ! P  |= (trm_app t1 t2) ~: T
-  | typing_trm_unit : forall E P,
+      E ! Y |= (trm_fvar x) ~: T
+  | typing_abs : forall L E Y U T t1,
+      (forall x, x \notin L -> (E & x ~ U) ! Y  |= t1 ^ x ~: T) ->
+      E ! Y |= (trm_abs t1) ~: (typ_arrow U T)
+  | typing_app : forall T1 T2 E Y t1 t2,
+      E ! Y |= t1 ~: (typ_arrow T1 T2) -> E ! Y  |= t2 ~: T1 ->
+      E ! Y  |= (trm_app t1 t2) ~: T2
+  | typing_unit : forall E Y,
       ok E ->
-      E ! P |= trm_unit ~: typ_unit
-  | typing_loc : forall E P l T,
+      E ! Y |= trm_unit ~: typ_unit
+  | typing_int : forall E Y n,
       ok E ->
-      binds l T P ->
-      E ! P |= (trm_loc l) ~: (typ_ref T)
-  | typing_new : forall E P t1 T,
-      E ! P |= t1 ~: T ->
-      E ! P |= (trm_ref t1) ~: (typ_ref T)
-  | typing_get : forall E P t1 T,
-      E ! P |= t1 ~: (typ_ref T) ->
-      E ! P |= (trm_get t1) ~: T
-  | typing_set : forall E P t1 t2 T,
-      E ! P |= t1 ~: (typ_ref T) ->
-      E ! P |= t2 ~: T ->
-      E ! P |= (trm_set t1 t2) ~: typ_unit
+      E ! Y |= (trm_int n) ~: typ_int
+  | typing_loc : forall E Y l T,
+      ok E ->
+      binds l T Y ->
+      E ! Y |= (trm_loc l) ~: (typ_ref T)
+  | typing_ref : forall E Y t1 T,
+      E ! Y |= t1 ~: T ->
+      E ! Y |= (trm_ref t1) ~: (typ_ref T)
+  | typing_get : forall E Y t1 T,
+      E ! Y |= t1 ~: (typ_ref T) ->
+      E ! Y |= (trm_get t1) ~: T
+  | typing_set : forall E Y t1 t2 T,
+      E ! Y |= t1 ~: (typ_ref T) ->
+      E ! Y |= t2 ~: T ->
+      E ! Y |= (trm_set t1 t2) ~: typ_unit
+  | typing_rand : forall E Y t1,
+      E ! Y |= t1 ~: typ_int ->
+      E ! Y |= (trm_rand t1) ~: typ_int
 
-where "E ! P |= t ~: T" := (typing E P t T).
+where "E ! Y |= t ~: T" := (typing E Y t T).
 
 (** Typing store *)
 
-Definition sto_typing P mu :=
+Definition sto_typing Y mu :=
      sto_ok mu
-  /\ (forall l, l # mu -> l # P)
-  /\ (forall l T, binds l T P ->
+  /\ (forall l, l # mu -> l # Y)
+  /\ (forall l T, binds l T Y ->
         exists t, binds l t mu
-               /\ empty ! P |= t ~: T).
+               /\ empty ! Y |= t ~: T).
 
-Notation "P |== mu" := (sto_typing P mu) (at level 68).
-
+Notation "Y |== mu" := (sto_typing Y mu) (at level 68).
 
 (** Definition of values *)
 
@@ -152,8 +169,10 @@ Inductive value : trm -> Prop :=
   | value_abs : forall t1,
       term (trm_abs t1) ->
       value (trm_abs t1)
-  | value_trm_unit :
+  | value_unit :
       value trm_unit
+  | value_int : forall n,
+      value (trm_int n)
   | value_loc : forall l,
       value (trm_loc l).
 
@@ -168,7 +187,7 @@ Inductive red : conf -> conf -> Prop :=
       term (trm_abs t1) ->
       value t2 ->
       red (trm_app (trm_abs t1) t2, mu) (t1 ^^ t2, mu)
-  | red_new : forall mu t1 l,
+  | red_ref : forall mu t1 l,
       sto_ok mu ->
       value t1 ->
       l # mu ->
@@ -190,7 +209,7 @@ Inductive red : conf -> conf -> Prop :=
       value t1 ->
       red (t2, mu) (t2', mu') ->
       red (trm_app t1 t2, mu) (trm_app t1 t2', mu')
-  | red_new_1 : forall mu mu' t1 t1',
+  | red_ref_1 : forall mu mu' t1 t1',
       red (t1, mu) (t1', mu') ->
       red (trm_ref t1, mu) (trm_ref t1', mu')
   | red_get_1 : forall mu mu' t1 t1',
@@ -203,24 +222,56 @@ Inductive red : conf -> conf -> Prop :=
   | red_set_2 : forall mu mu' t1 t2 t2',
       value t1 ->
       red (t2, mu) (t2', mu') ->
-      red (trm_set t1 t2, mu) (trm_set t1 t2', mu').
+      red (trm_set t1 t2, mu) (trm_set t1 t2', mu')
+  | red_rand : forall mu n m,
+      sto_ok mu ->
+      (0 <= m < max 1 n) ->
+      red (trm_rand (trm_int n), mu) ((trm_int m), mu)
+  | red_rand_1 : forall mu mu' t1 t1',
+      red (t1, mu) (t1', mu') ->
+      red (trm_rand t1, mu) (trm_rand t1', mu').
 
 Notation "c --> c'" := (red c c') (at level 68).
 
-(** Goal is to prove preservation and progress *)
+(** The goal is to prove type soundness *)
 
-Definition preservation := forall P t t' mu mu' T,
-  empty ! P |= t ~: T ->
-  (t,mu) --> (t',mu') ->
-  P |== mu ->
-  exists P',
-     extends P P'
-  /\ empty ! P' |= t' ~: T
-  /\ P' |== mu'.
+(** [reds c c'] is the reflexive-transitive closure of [red] *)
 
-Definition progress := forall P t mu T,
-  empty ! P |= t ~: T ->
-  P |== mu ->
-     value t
-  \/ exists t', exists mu', (t,mu) --> (t',mu').
+Inductive reds : conf -> conf -> Prop :=
+  | reds_here : forall c,
+      term (fst c) ->
+      reds c c
+  | reds_step : forall c1 c2 c3,
+      red c1 c2 ->
+      reds c2 c3 ->
+      reds c1 c3.
+
+(** Terminal configuration *)
+
+Definition terminal_conf (c:conf) : Prop :=
+  value (fst c).
+
+(** Reducible configuration *)
+
+Definition reducible_conf (c:conf) : Prop :=
+  exists c', c --> c'.
+
+(** Safety of a configuration *)
+
+Definition safe_conf (c:conf) : Prop :=
+  forall c', reds c c' -> terminal_conf c' \/ reducible_conf c'.
+
+(** Well-typed configuration *)
+
+Definition typed_conf (c:conf) : Prop :=
+  let '(t,mu) := c in
+  exists Y T,
+     empty ! Y |= t ~: T
+  /\ Y |== mu.
+
+(** Type soundness: starting from a well-typed configuration,
+    all accessible configurations are safe *)
+
+Definition soundness : Prop :=
+  forall c, typed_conf c -> safe_conf c.
 
