ln/ML_Core_Infrastructure.v
@@ -99,7 +99,7 @@ Notation "[ z ~> u ] t" := (trm_subst z u t) (at level 68).
 (** * Tactics *)
 
 (* ********************************************************************** *)
-(** ** Instanciation of Tactics *)
+(** ** Instantiation of Tactics *)
 
 Ltac gather_vars :=
   let A := gather_vars_with (fun x : vars => x) in
