ln/ML_Soundness.v
@@ -10,12 +10,12 @@ Require Import ML_Definitions ML_Infrastructure.
 (* ********************************************************************** *)
 (** Typing schemes for expressions *)
 
-Definition has_scheme_vars L E P t M := forall Xs, 
+Definition has_scheme_vars L E P t M := forall Xs,
   fresh L (sch_arity M) Xs ->
   E ! P |= t ~: (M ^ Xs).
 
 Definition has_scheme E P t M := forall Vs,
-  types (sch_arity M) Vs -> 
+  types (sch_arity M) Vs ->
   E ! P |= t ~: (M ^^ Vs).
 
 (* ********************************************************************** *)
@@ -26,14 +26,14 @@ Lemma pat_typing_typ_subst : forall Z U Us p T,
   LibList.map (typ_subst Z U) Us \= p ~: typ_subst Z U T.
 Proof.
   induction 1; simpls*. rew_listx; auto. rew_listx; auto.
-Qed.  
+Qed.
 
 (* ********************************************************************** *)
 (** Type substitution preserves typing of expressions *)
 
 Lemma typing_typ_subst : forall F P Z U E t T,
-  Z \notin (env_fv E) -> Z \notin (phi_fv P) -> type U -> 
-  E & F ! P |= t ~: T -> 
+  Z \notin (env_fv E) -> Z \notin (phi_fv P) -> type U ->
+  E & F ! P |= t ~: T ->
   E & (map (sch_subst Z U) F) ! P |= t ~: (typ_subst Z U T).
 Proof.
   introv. intros Fr1 Fr2 WVs Typ. gen_eq G: (E & F). gen F.
@@ -45,7 +45,7 @@ Proof.
       autos*.
     rewrite~ sch_subst_arity. apply* typ_subst_type_list.
   apply_fresh* typing_abs. intros y Fr.
-   rewrite sch_subst_fold.   
+   rewrite sch_subst_fold.
    apply_ih_map_bind* H1.
   apply_fresh* typing_fix. intros f y Fr.
    applys_eq* H1 4. do 2 rewrite <- concat_assoc. fequal.
@@ -54,10 +54,10 @@ Proof.
   apply_fresh* (@typing_let (sch_subst Z U M) (L1 \u \{Z})).
    simpl. intros Ys Fr. rewrite* <- sch_subst_open_vars.
    intros y Fr. apply_ih_map_bind* H4.
-  apply_fresh* (@typing_match (typ_subst Z U T) 
+  apply_fresh* (@typing_match (typ_subst Z U T)
                               (LibList.map (typ_subst Z U) Us)).
     apply* pat_typing_typ_subst.
-    intros xs Fr. 
+    intros xs Fr.
      rewrite factorize_map; [| apply* pat_typing_arity_elim ].
      rewrite <- concat_assoc. rewrite <- map_concat.
      apply* H1. rewrite* concat_assoc.
@@ -74,22 +74,22 @@ Proof.
   autos*.
   apply* typing_set.
   apply* typing_raise.
-   rewrite* <- (@typ_subst_fresh Z U typ_exn). 
-  apply* typing_catch. 
-   rewrite* <- (@typ_subst_fresh Z U typ_exn). 
+   rewrite* <- (@typ_subst_fresh Z U typ_exn).
+  apply* typing_catch.
+   rewrite* <- (@typ_subst_fresh Z U typ_exn).
 Qed.
 
 (* ********************************************************************** *)
 (** Iterated type substitution preserves typing *)
 
 Lemma typing_typ_substs : forall Zs Us E P t T,
-  fresh (env_fv E \u phi_fv P) (length Zs) Zs -> 
+  fresh (env_fv E \u phi_fv P) (length Zs) Zs ->
   types (length Zs) Us ->
-  E ! P |= t ~: T -> 
+  E ! P |= t ~: T ->
   E ! P |= t ~: (typ_substs Zs Us T).
 Proof.
   induction Zs; destruct Us; simpl; introv Fr WU Tt;
-   destruct Fr; inversions WU; 
+   destruct Fr; inversions WU;
    simpls; try solve [ auto | false* ].
   inverts H2. inverts H1.
   apply* IHZs. apply_empty* typing_typ_subst.
@@ -114,7 +114,7 @@ Qed.
 (** A term that has type T has type scheme "forall(no_var).T" *)
 
 Lemma has_scheme_from_typ : forall E P t T,
-  E ! P |= t ~: T -> 
+  E ! P |= t ~: T ->
   has_scheme E P t (Sch 0 T).
 Proof.
   intros_all. unfold sch_open. simpls. rewrite* <- typ_open_type.
@@ -124,14 +124,14 @@ Qed.
 (** Typing is preserved by weakening *)
 
 Lemma typing_weaken : forall G E F P t T,
-   (E & G) ! P |= t ~: T -> 
+   (E & G) ! P |= t ~: T ->
    ok (E & F & G) ->
    (E & F & G) ! P |= t ~: T.
 Proof.
   introv Typ. gen_eq H: (E & G). gen G.
   induction Typ; intros G EQ Ok; subst.
   apply* typing_var. apply* binds_weaken.
-  apply_fresh* typing_abs. intros y Fr. 
+  apply_fresh* typing_abs. intros y Fr.
    do_rew* concat_assoc (apply* H1).
   apply_fresh* typing_fix. intros f y Fr2.
    do_rew_2 concat_assoc (apply* H1). auto. auto.
@@ -139,7 +139,7 @@ Proof.
    do_rew* concat_assoc (apply* H4).
   apply_fresh* (@typing_match T Us). intros xs Fr.
     do_rew* concat_assoc (apply* H1).
-    apply* (@ok_singles sch (pat_arity p)). 
+    apply* (@ok_singles sch (pat_arity p)).
     do 2 rewrite dom_concat. auto.
     rewrite length_map. apply* pat_typing_arity_elim.
   autos*.
@@ -160,7 +160,7 @@ Qed.
 (* ********************************************************************** *)
 (** Values are preserved by term substitution *)
 
-Lemma value_fv : forall z u t, 
+Lemma value_fv : forall z u t,
   value u -> value t -> value ([z ~> u]t).
 Proof.
   introv Valu Valt. induction Valt; simpls*.
@@ -169,13 +169,13 @@ Qed.
 (* ********************************************************************** *)
 (** Typing is preserved by term substitution *)
 
-Lemma typing_trm_subst : forall F M E P t T z u, 
+Lemma typing_trm_subst : forall F M E P t T z u,
   E & z ~ M & F ! P |= t ~: T ->
-  has_scheme E P u M -> 
+  has_scheme E P u M ->
   value u ->
   E & F ! P |= (trm_subst z u t) ~: T.
 Proof.
-  introv Typt. intros Typu Valu. 
+  introv Typt. intros Typu Valu.
   gen_eq G: (E & z ~ M & F). gen F.
   induction Typt; intros G EQ; subst; simpl trm_subst.
   case_var.
@@ -188,7 +188,7 @@ Proof.
    rewrite* subst_open_vars.
    do_rew_2 concat_assoc (apply* H1). auto.
   apply_fresh* (@typing_let M0 L1); try intros y Fr.
-   apply* value_fv. 
+   apply* value_fv.
    rewrite* subst_open_vars. do_rew* concat_assoc (apply* H4).
   apply_fresh* (@typing_match T Us). intros xs Fr.
    rewrite* subst_open_vars.
@@ -220,13 +220,13 @@ Lemma typing_trm_substs : forall Us E P xs ts t T,
 Proof.
   introv EQ Typts Typt Val. gen Us ts t T.
   induction xs; destruct ts; intros; tryfalse.
-  inversions Typts. inversions Val. rew_listx in Typt. 
+  inversions Typts. inversions Val. rew_listx in Typt.
    rewrite singles_nil,concat_empty_r in Typt. auto.
   rew_list in EQ. inverts EQ as EQ.
-   inversions Typts. inversions Val. rew_listx in Typt. 
+   inversions Typts. inversions Val. rew_listx in Typt.
    rewrite singles_cons in Typt. rewrite concat_assoc in Typt.
    simpl. apply* (@IHxs Us0).
-   apply_empty* typing_trm_subst. 
+   apply_empty* typing_trm_subst.
    apply* has_scheme_from_typ. apply_empty* typing_weaken.
    lets~ : (proj1 (typing_regular Typt)).
 Qed.
@@ -240,10 +240,10 @@ Lemma typing_pattern_match : forall p t T E P ts Us,
   Us \= p ~: T ->
   typings E P ts Us.
 Proof.
-  induction p; introv H1 H2 H0; destruct t; 
+  induction p; introv H1 H2 H0; destruct t;
    inversion H0; inversion H1; auto; subst; inversions H2; autos*.
-  remember (pat_match p1 t1) as K1. 
-   remember (pat_match p2 t2) as K2. 
+  remember (pat_match p1 t1) as K1.
+   remember (pat_match p2 t2) as K2.
    destruct K1 as [ts1|]; destruct K2 as [ts2|]; try discriminate.
    inversions H9. apply* typings_concat.
 Qed.
@@ -256,30 +256,30 @@ Lemma pattern_match_values : forall p t ts,
   value t ->
   Forall value ts.
 Proof.
-  induction p; introv EQ Val; 
+  induction p; introv EQ Val;
    destruct t; simpl in EQ; inversion EQ; auto; inversions Val; autos*.
-  remember (pat_match p1 t1) as K1. 
-   remember (pat_match p2 t2) as K2. 
+  remember (pat_match p1 t1) as K1.
+   remember (pat_match p2 t2) as K2.
    destruct K1 as [ts1|]; destruct K2 as [ts2|]; try discriminate.
    inversions EQ. apply* Forall_app.
 Qed.
 
 (* ********************************************************************** *)
-(** Typing is preserved by an extension of store typing. 
+(** Typing is preserved by an extension of store typing.
     (This result is added to hints because we use it many times. *)
 
 Lemma typing_stability : forall P E P' t T,
   E ! P |= t ~: T ->
-  extends P P' -> 
+  extends P P' ->
   phi_ok P' ->
   E ! P' |= t ~: T.
 Proof.
   introv Typ Ext. induction Typ.
   autos*.
-  autos*. 
+  autos*.
 intros.
-clear H0. 
-(* eauto.  
+clear H0.
+(* eauto.
  (* COQBUG*) *)
 
 (* was: induction* Typ. *)
@@ -299,20 +299,20 @@ Proof.
   unfold sto_typing. introv [PhiOk [StoOk [Dom Ext]]]. splits 4.
     auto.
     auto.
-    intros l0 Fr. simpls. lets: (Dom l0). 
+    intros l0 Fr. simpls. lets: (Dom l0).
       asserts* Frl0: (l0 # P). auto.
     intros l' T' Has. binds_cases Has.
       destruct (Ext _ _ B) as [t' [Hast' Typt']].
-       exists* t'. 
+       exists* t'.
       subst. exists* t.
-Qed.   
+Qed.
 
 (* ********************************************************************** *)
 (** Fails always returns an exception. *)
 
 Lemma fails_to_exception : forall E P t T e,
-  fails t e -> 
-  E ! P |= t ~: T -> 
+  fails t e ->
+  E ! P |= t ~: T ->
   E ! P |= e ~: typ_exn.
 Proof.
   introv Fail Typ. induction Typ; inversions* Fail.
@@ -328,15 +328,15 @@ Ltac pres H t' mu' :=
   let Ext := fresh "Ext" in
   let Typt' := fresh "Typt'" in
   let TypSto' := fresh "TypSto'" in
-  destruct~ (H (@refl_equal env empty) t' mu') 
-                  as [P' [Ext [Typt' TypSto']]].  
+  destruct~ (H (@refl_equal env empty) t' mu')
+                  as [P' [Ext [Typt' TypSto']]].
 
 Lemma preservation_result : preservation.
 Proof.
   introv Typ. gen t' mu'. gen_eq E: (empty : env).
-  induction Typ; intros EQ t' mu' Red TypSto; subst; 
-   inversions Red. 
-  exists P. splits~ 3. 
+  induction Typ; intros EQ t' mu' Red TypSto; subst;
+   inversions Red.
+  exists P. splits~ 3.
    pick_fresh x. forwards~ K: (H3 x). clear H2 H3 H4.
    rewrite~ (@substs_intro (x::nil)).
      simpl. apply_empty* typing_trm_subst.
@@ -347,22 +347,22 @@ Proof.
    pick_freshes (pat_arity p) xs.
    rewrite~ (@substs_intro xs);
     [| rewrite~ <- (fresh_length Fr)].
-   forwards~ K: (H0 xs). 
-   rewrite (proj1 Wts) in Fr, Wts.
-   apply_empty* (@typing_trm_substs Us). 
+   forwards~ K: (H0 xs).
+   lets E: (proj1 Wts). rewrite E in Fr, Wts.
+   apply_empty* (@typing_trm_substs Us).
      rewrite* (fresh_length Fr).
      apply* typing_pattern_match.
      apply* pattern_match_values.
   exists P. splits~ 3.
   pres IHTyp1 t1' mu'. exists* P'.
-  exists P. splits~ 3. 
-   inversions Typ1. 
+  exists P. splits~ 3.
+   inversions Typ1.
    pick_fresh x. forwards~ K: (H8 x). clear H8 IHTyp1 IHTyp2.
    rewrite~ (@substs_intro (x::nil)).
      simpl. apply_empty* typing_trm_subst.
       apply* has_scheme_from_typ.
      rewrite trm_fv_list_cons, trm_fv_list_nil. rew_list~.
-  exists P. splits~ 3. 
+  exists P. splits~ 3.
    inversions Typ1.
    pick_fresh f. pick_fresh x. rewrite~ (@substs_intro (x::f::nil)).
     apply_empty* (@typing_trm_substs (S::(typ_arrow S T)::nil)).
@@ -377,21 +377,21 @@ Proof.
   pres IHTyp t1' mu'. exists* P'.
   pres IHTyp t1' mu'. exists* P'.
   exists (P & l ~ T). lets: (proj43 TypSto).
-   splits~ 3. apply* sto_typing_push. 
-  pres IHTyp t1' mu'. exists* P'. 
-  exists P. splits~ 3. 
-   inversions Typ. 
+   splits~ 3. apply* sto_typing_push.
+  pres IHTyp t1' mu'. exists* P'.
+  exists P. splits~ 3.
+   inversions Typ.
    destruct~ ((proj44 TypSto) l T) as [t [Hast Typt]].
    rewrite~ (binds_functional H4 Hast).
   pres IHTyp t1' mu'. exists* P'.
-  exists P. inversions Typ1. splits~ 3. 
+  exists P. inversions Typ1. splits~ 3.
    destruct TypSto as [PhiOk [StoOk [Dom Map]]]. splits~ 4.
-    intros. tests: (l = l0). 
+    intros. tests: (l = l0).
       exists t2. split~. rewrite~ (binds_functional H H7).
-      destruct (Map _ _ H) as [t [Has Typ]]. exists* t.  
+      destruct (Map _ _ H) as [t [Has Typ]]. exists* t.
   pres IHTyp1 t1' mu'. exists* P'.
   pres IHTyp2 t2' mu'. exists* P'.
-  pres IHTyp t1' mu'. exists* P'. 
+  pres IHTyp t1' mu'. exists* P'.
   exists* P.
   exists P. splits~ 3.
     apply* typing_app. apply* fails_to_exception.
@@ -416,7 +416,7 @@ Hint Constructors fails.
 Lemma progress_result : progress.
 Proof.
   introv Typ. gen_eq E: (empty:env). lets Typ': Typ.
-  induction Typ; intros; subst. 
+  induction Typ; intros; subst.
   false* binds_empty_inv.
   branch* 1.
   branch* 1.
@@ -425,30 +425,30 @@ Proof.
     forwards~ [Val1 | [[e Fail] | [t1' [mu' Red1]]]]: (@H2 Ys).
      branch 3. exists* (t2 ^^ (t1::nil)) mu.
      branch 2. exists* e.
-     false. apply* (red_value_false H Red1). 
+     false. apply* (red_value_false H Red1).
   destruct~ IHTyp1 as [Val1 | [[e Fail] | [t1' [mu' Red1]]]].
     branch 3. remember (pat_match p t1) as K. destruct K as [ts|].
       exists* (b ^^ ts) mu.
       exists* t2 mu.
-    branch 2. exists* e. 
+    branch 2. exists* e.
     branch 3. exists* (trm_match t1' p b t2) mu'.
   destruct~ IHTyp1 as [Val1 | [[e Fail] | [t1' [mu' Red1]]]].
     destruct~ IHTyp2 as [Val2 | [[e Fail] | [t2' [mu' Red2]]]].
-      inversions Typ1; inversion Val1. 
+      inversions Typ1; inversion Val1.
         branch 3. exists* (t0 ^^ (t2::nil)) mu.
-        branch 3. exists* (t0 ^^ (t2::(trm_fix t0)::nil)) mu. 
-        branch 3. subst. inversions H1. inversions H0. inversions Val2; inversions Typ2. 
+        branch 3. exists* (t0 ^^ (t2::(trm_fix t0)::nil)) mu.
+        branch 3. subst. inversions H1. inversions H0. inversions Val2; inversions Typ2.
            exists* (trm_nat (n + n0)) mu.
            inversions H5.
-        branch 1. inversions Val2; inversions Typ2. 
+        branch 1. inversions Val2; inversions Typ2.
           autos*.
           inversions H4.
         branch 2. exists* e.
         branch 3. exists* (trm_app t1 t2') mu'.
-    branch 2. exists* e. 
+    branch 2. exists* e.
     branch 3. exists* (trm_app t1' t2) mu'.
   branch* 1.
-  branch* 1.  
+  branch* 1.
   branch* 1.
   destruct~ IHTyp1 as [Val1 | [[e Fail] | [t1' [mu' Red1]]]].
     destruct~ IHTyp2 as [Val2 | [[e Fail] | [t2' [mu' Red2]]]].
@@ -467,32 +467,32 @@ Proof.
     destruct (var_fresh (dom mu)) as [l Fr].
       branch 3. exists* (trm_loc l) (mu & l ~ t1).
       branch 2. exists* e.
-    branch 3. exists* (trm_ref t1') mu'. 
+    branch 3. exists* (trm_ref t1') mu'.
   destruct~ IHTyp as [Val1 | [[e Fail] | [t1' [mu' Red1]]]].
     inversions Val1; inversions Typ.
-      inversion H4.  
+      inversion H4.
       destruct ((proj44 H) _ _ H6) as [t' [Has' Typt']].
        branch 3. exists* t' mu.
     branch 2. exists* e.
     branch 3. exists* (trm_get t1') mu'.
   destruct~ IHTyp1 as [Val1 | [[e Fail] | [t1' [mu' Red1]]]].
     destruct~ IHTyp2 as [Val2 | [[e Fail] | [t2' [mu' Red2]]]].
-      inversions Val1; inversions Typ1.  
+      inversions Val1; inversions Typ1.
         inversion H4.
         destruct ((proj44 H) _ _ H6) as [t' [Has' Typt']].
          branch 3. exists* trm_unit (mu & l ~ t2).
-      branch 2. exists* e. 
-      branch 3. exists* (trm_set t1 t2') mu'. 
+      branch 2. exists* e.
+      branch 3. exists* (trm_set t1 t2') mu'.
     branch 2. exists* e.
     branch 3. exists* (trm_set t1' t2) mu'.
   destruct~ IHTyp as [Val1 | [[e Fail] | [t1' [mu' Red1]]]].
-    branch 2. exists* t1. 
-    branch 2. exists* e. 
-    branch 3. exists* (trm_raise t1') mu'. 
+    branch 2. exists* t1.
+    branch 2. exists* e.
+    branch 3. exists* (trm_raise t1') mu'.
   destruct~ IHTyp2 as [Val2 | [[e Fail] | [t2' [mu' Red2]]]].
-    branch 3. exists* t2 mu. 
+    branch 3. exists* t2 mu.
     branch 3. exists* (trm_app t1 e) mu.
-    branch 3. exists* (trm_catch t1 t2') mu'. 
+    branch 3. exists* (trm_catch t1 t2') mu'.
 Qed.
 
 
