ln/STLC_Core_WF_Infrastructure.v
@@ -39,7 +39,7 @@ Definition body t :=
 
 
 (* ********************************************************************** *)
-(** ** Instanciation of Tactics *)
+(** ** Instantiation of Tactics *)
 
 Ltac gather_vars :=
   let A := gather_vars_with (fun x : vars => x) in
