ln/STLC_Mut_Infrastructure.v
@@ -47,7 +47,7 @@ Definition body t :=
 
 
 (* ********************************************************************** *)
-(** ** Instanciation of tactics *)
+(** ** Instantiation of tactics *)
 
 (** Tactic [gather_vars] returns a set of variables occurring in
     the context of proofs, including domain of environments and
