README.md
@@ -1,48 +1,59 @@
-# Arthur Charguéraud's Formal Metatheory in Coq
+# Arthur Charguéraud's Archive of Formal Metatheory in Coq
+
+This repository contains a collection of formalizations
+of programming language semantics and type soundness proofs.
+
+Feel free to use them as templates for your own developments.
 
 
-Description
-===========
+Contents
+========
 
    - Folder `ln` contains locally nameless developments.
-     See the paper "The Locally Nameless Representation" (JAR'11)
+     See the paper "The Locally Nameless Representation" (JAR'11).
      http://www.chargueraud.org/research/2009/ln/main.pdf
 
    - Folder `pretty` contains pretty-big-step developments.
-     See the paper Pretty Big Step Semantics (ESOP'13)
+     See the Pretty-Big-Step paper (ESOP'13).
      http://www.chargueraud.org/research/2012/pretty/pretty.pdf
 
-   - Folder `Tuto` contains course notes:
+   - Folder `omni` formalizes omni-big-step and omni-small-step.
+     See the Omni-Semantics paper (TOPLAS'23).
+     http://www.chargueraud.org/research/2022/omnisemantics/omnisemantics.pdf
 
-      + File `Classic` is a tutorial on using classical logic in Coq
-
-      + File `Coind` are incomplete notes on coinduction
+   - Folder `tuto` contains a tutorial on the use of classical logic in Coq.
 
 
 Compilation
 ===========
 
-The files should compile with Coq v8.15.
+The files compile with Coq v8.18.
 
-The compilation of the files depends on the TLC library.
-TLC is available from `opam`, package named `coq-tlc`.
+A tutorial on how to best configure Coq in VScode is available from:
+https://chargueraud.org/teach/verif/install/install.html
 
-TLC can also be installed by hand.
+The compilation of the files depends on the TLC library, available from `opam`.
+
+```
+  opam install coq-tlc
+```
+
+Alternatively, TLC may be installed by hand.
 
 ```
   git clone git@github.com:charguer/tlc.git
-  cd src
-  make install
+  make -j4 all && make install
 ```
 
-The command for compiling all files:
+To play the files interactively, enter one of the subfolders, compile
+the scripts, then edit them, e.g., in VScode:
 
 ```
-   make -j4 all
+  cd ln
+  make -j4
+  code . &
 ```
 
-The command `make -j4 vos` processes all files in a faster way,
-to make them ready for interactive use.
 
 
 License
@@ -53,4 +64,5 @@ All files are distributed under the MIT X11 license. See the LICENSE file.
 Authors
 =======
 
-See the AUTHORS file.
+All files in this repository are authored by Arthur Charguéraud.
+
