pretty/open.sh
@@ -1,7 +1,0 @@
-COQBIN=
-TLC=
-if [ -f settings.sh ]
-then
-    source settings.sh
-fi
-${COQBIN}coqide -async-proofs off -async-proofs-command-error-resilience off -R ${TLC} TLC -R . PRETTY $*
